Rename interp_op to apply_op

Move.thy
@@ -47,36 +47,37 @@ fun redo_op :: \<open>('t, 'n, 'm) log_op \<Rightarrow> ('t, 'n, 'm) state \<Rig
      (let (op2, tree2) = do_op (Move t p m c, tree)
       in (op2 # ops, tree2))\<close>
 
-fun interp_op :: \<open>('t::{linorder}, 'n, 'm) operation \<Rightarrow>
+fun apply_op :: \<open>('t::{linorder}, 'n, 'm) operation \<Rightarrow>
                   ('t, 'n, 'm) state \<Rightarrow> ('t, 'n, 'm) state\<close> where
-  \<open>interp_op op1 ([], tree1) =
+  \<open>apply_op op1 ([], tree1) =
      (let (op2, tree2) = do_op (op1, tree1)
       in ([op2], tree2))\<close> |
-  \<open>interp_op op1 (logop # ops, tree1) =
+  \<open>apply_op op1 (logop # ops, tree1) =
      (if move_time op1 < log_time logop
-      then redo_op logop (interp_op op1 (ops, undo_op (logop, tree1)))
+      then redo_op logop (apply_op op1 (ops, undo_op (logop, tree1)))
       else let (op2, tree2) = do_op (op1, tree1) in (op2 # logop # ops, tree2))\<close>
 
-abbreviation interp_ops' :: \<open>('t::{linorder}, 'n, 'm) operation list \<Rightarrow> ('t, 'n, 'm) state \<Rightarrow> ('t, 'n, 'm) state\<close> where
-  \<open>interp_ops' ops initial \<equiv> foldl (\<lambda>state oper. interp_op oper state) initial ops\<close>
+abbreviation apply_ops' :: \<open>('t::{linorder}, 'n, 'm) operation list \<Rightarrow> ('t, 'n, 'm) state \<Rightarrow> ('t, 'n, 'm) state\<close> where
+  \<open>apply_ops' ops initial \<equiv> foldl (\<lambda>state oper. apply_op oper state) initial ops\<close>
 
-definition interp_ops :: \<open>('t::{linorder}, 'n, 'm) operation list \<Rightarrow> ('t, 'n, 'm) state\<close>
-  where \<open>interp_ops ops \<equiv> interp_ops' ops ([], {})\<close>
+definition apply_ops :: \<open>('t::{linorder}, 'n, 'm) operation list \<Rightarrow> ('t, 'n, 'm) state\<close>
+  where \<open>apply_ops ops \<equiv> apply_ops' ops ([], {})\<close>
 
 definition unique_parent :: \<open>('n \<times> 'm \<times> 'n) set \<Rightarrow> bool\<close> where
   \<open>unique_parent tree \<equiv> (\<forall>p1 p2 m1 m2 c. (p1, m1, c) \<in> tree \<and> (p2, m2, c) \<in> tree \<longrightarrow> p1 = p2 \<and> m1 = m2)\<close>
-lemma interp_ops_base [simp]:
-  shows \<open>interp_ops [Move t1 p1 m1 c1, Move t2 p2 m2 c2] =
-                    interp_op (Move t2 p2 m2 c2) (interp_op (Move t1 p1 m1 c1) ([], {}))\<close>
-  by (clarsimp simp add: interp_ops_def)
 
-lemma interp_ops_step [simp]:
-  shows \<open>interp_ops (xs @ [x]) = interp_op x (interp_ops xs)\<close>
-  by (clarsimp simp add: interp_ops_def)
+lemma apply_ops_base [simp]:
+  shows \<open>apply_ops [Move t1 p1 m1 c1, Move t2 p2 m2 c2] =
+                    apply_op (Move t2 p2 m2 c2) (apply_op (Move t1 p1 m1 c1) ([], {}))\<close>
+  by (clarsimp simp add: apply_ops_def)
 
-lemma interp_ops_Nil [simp]:
-  shows \<open>interp_ops [] = ([], {})\<close>
-  by (clarsimp simp add: interp_ops_def)
+lemma apply_ops_step [simp]:
+  shows \<open>apply_ops (xs @ [x]) = apply_op x (apply_ops xs)\<close>
+  by (clarsimp simp add: apply_ops_def)
+
+lemma apply_ops_Nil [simp]:
+  shows \<open>apply_ops [] = ([], {})\<close>
+  by (clarsimp simp add: apply_ops_def)
 
 section \<open>undo-op is the inverse of do-op\<close>
 
@@ -246,16 +247,16 @@ proof -
     by (metis assms(1) do_op_unique_parent)
 qed
 
-lemma interp_op_unique_parent:
+lemma apply_op_unique_parent:
   assumes \<open>unique_parent tree1\<close>
-    and \<open>interp_op oper (ops1, tree1) = (ops2, tree2)\<close>
+    and \<open>apply_op oper (ops1, tree1) = (ops2, tree2)\<close>
   shows \<open>unique_parent tree2\<close>
 using assms proof(induct ops1 arbitrary: tree1 tree2 ops2)
   case Nil
   have \<open>\<And>pair. snd (case pair of (p1, p2) \<Rightarrow> ([p1], p2)) = snd pair\<close>
     by (simp add: prod.case_eq_if)
   hence \<open>\<exists>log_op. do_op (oper, tree1) = (log_op, tree2)\<close>
-    by (metis Nil.prems(2) interp_op.simps(1) prod.collapse snd_conv)
+    by (metis Nil.prems(2) apply_op.simps(1) prod.collapse snd_conv)
   thus \<open>unique_parent tree2\<close>
     by (metis Nil.prems(1) do_op_unique_parent operation.exhaust_sel)
 next
@@ -267,42 +268,42 @@ next
       by simp
     moreover from this have 1: \<open>unique_parent tree1a\<close>
       using undo_op_unique_parent by (metis step.prems(1) log_op.exhaust_sel)
-    moreover obtain ops1b tree1b where \<open>(ops1b, tree1b) = interp_op oper (ops, tree1a)\<close>
+    moreover obtain ops1b tree1b where \<open>(ops1b, tree1b) = apply_op oper (ops, tree1a)\<close>
       by (metis surj_pair)
     moreover from this have \<open>unique_parent tree1b\<close>
       using 1 by (metis step.hyps)
     ultimately show \<open>unique_parent tree2\<close>
-      using redo_op_unique_parent by (metis interp_op.simps(2) step.prems(2))
+      using redo_op_unique_parent by (metis apply_op.simps(2) step.prems(2))
   next
     case False
     hence \<open>snd (do_op (oper, tree1)) = tree2\<close>
-      by (metis (mono_tags, lifting) interp_op.simps(2) prod.sel(2) split_beta step.prems(2))
+      by (metis (mono_tags, lifting) apply_op.simps(2) prod.sel(2) split_beta step.prems(2))
     then show \<open>unique_parent tree2\<close>
       by (metis do_op_unique_parent operation.exhaust_sel prod.exhaust_sel step.prems(1))
   qed
 qed
 
-theorem interp_ops_unique_parent:
-  assumes \<open>interp_ops ops = (log, tree)\<close>
+theorem apply_ops_unique_parent:
+  assumes \<open>apply_ops ops = (log, tree)\<close>
   shows \<open>unique_parent tree\<close>
 using assms proof(induction ops arbitrary: log tree rule: List.rev_induct)
   case Nil
-  hence \<open>interp_ops [] = ([], {})\<close>
-    by (simp add: interp_ops_def)
+  hence \<open>apply_ops [] = ([], {})\<close>
+    by (simp add: apply_ops_def)
   hence \<open>tree = {}\<close>
     by (metis Nil.prems snd_conv)
   then show ?case
     by (simp add: unique_parent_def)
 next
   case (snoc x xs)
-  obtain log tree where interp_xs: \<open>interp_ops xs = (log, tree)\<close>
+  obtain log tree where apply_xs: \<open>apply_ops xs = (log, tree)\<close>
     by fastforce
-  hence \<open>interp_ops (xs @ [x]) = interp_op x (log, tree)\<close>
-    by (simp add: interp_ops_def)
+  hence \<open>apply_ops (xs @ [x]) = apply_op x (log, tree)\<close>
+    by (simp add: apply_ops_def)
   moreover have \<open>unique_parent tree\<close>
-    by (simp add: interp_xs snoc.IH)
+    by (simp add: apply_xs snoc.IH)
   ultimately show ?case
-    by (metis interp_op_unique_parent snoc.prems)
+    by (metis apply_op_unique_parent snoc.prems)
 qed
 
 
@@ -652,8 +653,8 @@ lemma undo_op_acyclic:
 
 lemma
   assumes \<open>\<not> cyclic tree1\<close>
-    and \<open>\<forall>log1 tree1 log2 tree2. interp_op x (log1, tree1) = (log2, tree2) \<and> \<not> cyclic tree1 \<longrightarrow> \<not> cyclic tree2\<close>
-    and \<open>redo_op a (interp_op x (log1, undo_op (a, tree1))) = (log2, tree2)\<close>
+    and \<open>\<forall>log1 tree1 log2 tree2. apply_op x (log1, tree1) = (log2, tree2) \<and> \<not> cyclic tree1 \<longrightarrow> \<not> cyclic tree2\<close>
+    and \<open>redo_op a (apply_op x (log1, undo_op (a, tree1))) = (log2, tree2)\<close>
   shows \<open>\<not> cyclic tree2\<close>
   using assms
   apply (induction log1 arbitrary: a tree1 log2 tree2)
@@ -685,12 +686,12 @@ lemma
 
 
 (*
-lemma \<open>\<exists>log2. redo_op a (interp_op x (log1, undo_op (a, tree1))) = (log2, tree1)\<close>
+lemma \<open>\<exists>log2. redo_op a (apply_op x (log1, undo_op (a, tree1))) = (log2, tree1)\<close>
   *)
 
-lemma interp_op_acyclic:
+lemma apply_op_acyclic:
   assumes \<open>\<not> cyclic tree1\<close>
-    and \<open>interp_op x (log1, tree1) = (log2, tree2)\<close>
+    and \<open>apply_op x (log1, tree1) = (log2, tree2)\<close>
   shows \<open>\<not> cyclic tree2\<close>
   using assms
   apply (induction log1 arbitrary: log2 tree1 tree2)
@@ -710,7 +711,7 @@ lemma interp_op_acyclic:
   apply clarsimp
   apply (case_tac x2)
    apply clarsimp
-   apply (case_tac "interp_op x (log1, {(p', m', c'). (p', m', c') \<in> tree1 \<and> c' \<noteq> x5})")
+   apply (case_tac "apply_op x (log1, {(p', m', c'). (p', m', c') \<in> tree1 \<and> c' \<noteq> x5})")
    apply (erule_tac x=a in meta_allE)
    apply (erule_tac x="{(p', m', c'). (p', m', c') \<in> tree1 \<and> c' \<noteq> x5}" in meta_allE)
    apply (erule_tac x=b in meta_allE)
@@ -727,14 +728,14 @@ lemma interp_op_acyclic:
 
 
 
-theorem interp_ops_acyclic:
-  assumes \<open>interp_ops ops = (log, tree)\<close>
+theorem apply_ops_acyclic:
+  assumes \<open>apply_ops ops = (log, tree)\<close>
   shows \<open>\<not> cyclic tree\<close>
   using assms
   apply (induction ops arbitrary: log tree rule: List.rev_induct)
    apply force
   apply simp
-  apply (case_tac "interp_ops xs")
+  apply (case_tac "apply_ops xs")
   apply (erule_tac x=a in meta_allE)
   apply (erule_tac x=b in meta_allE)
   apply clarsimp
@@ -750,15 +751,15 @@ theorem interp_ops_acyclic:
 (*
 using assms proof(induction ops arbitrary: log tree rule: List.rev_induct)
   case Nil
-  then show ?case by (simp add: cyclic_def interp_ops_def)
+  then show ?case by (simp add: cyclic_def apply_ops_def)
 next
   case (snoc x xs)
-  then obtain log1 tree1 where \<open>interp_ops xs = (log1, tree1)\<close>
+  then obtain log1 tree1 where \<open>apply_ops xs = (log1, tree1)\<close>
     by fastforce
-  moreover from this have \<open>interp_ops (xs @ [x]) = interp_op x (log1, tree1)\<close>
-    by simp
+  moreover from this have \<open>apply_ops (xs @ [x]) = apply_op x (log1, tree1)\<close>
+    by (metis (no_types) foldl_Cons foldl_Nil foldl_append apply_ops_def)
   ultimately show ?case
-    sorry (* TODO: need to generalise do_op_acyclic to hold for interp_op *)
+    sorry (* TODO: need to generalise do_op_acyclic to hold for apply_op *)
 qed
 *)
 
@@ -770,11 +771,11 @@ lemma distinct_list_pick1:
   shows \<open>set xs = set (ys @ zs)\<close>
 using assms by (induction xs) (fastforce+)
 
-lemma interp_op_commute_base:
+lemma apply_op_commute_base:
   assumes \<open>t1 < t2\<close>
     and \<open>unique_parent tree\<close>
-  shows \<open>interp_op (Move t2 p2 m2 c2) (interp_op (Move t1 p1 m1 c1) ([], tree)) =
-         interp_op (Move t1 p1 m1 c1) (interp_op (Move t2 p2 m2 c2) ([], tree))\<close>
+  shows \<open>apply_op (Move t2 p2 m2 c2) (apply_op (Move t1 p1 m1 c1) ([], tree)) =
+         apply_op (Move t1 p1 m1 c1) (apply_op (Move t2 p2 m2 c2) ([], tree))\<close>
 proof -
   obtain tree1 where tree1: \<open>do_op (Move t1 p1 m1 c1, tree) =
       (LogMove t1 (get_parent tree c1) p1 m1 c1, tree1)\<close>
@@ -789,21 +790,21 @@ proof -
     using assms(2) do_undo_op_inv by fastforce
   have \<open>\<not> t2 < t1\<close>
     using not_less_iff_gr_or_eq assms(1) by blast
-  hence \<open>interp_op (Move t2 p2 m2 c2) (interp_op (Move t1 p1 m1 c1) ([], tree)) =
+  hence \<open>apply_op (Move t2 p2 m2 c2) (apply_op (Move t1 p1 m1 c1) ([], tree)) =
         ([LogMove t2 (get_parent tree1 c2) p2 m2 c2, LogMove t1 (get_parent tree c1) p1 m1 c1], tree12)\<close>
     using tree1 tree12 by auto
-  moreover have \<open>interp_op (Move t2 p2 m2 c2) ([], tree) =
+  moreover have \<open>apply_op (Move t2 p2 m2 c2) ([], tree) =
       ([LogMove t2 (get_parent tree c2) p2 m2 c2], tree2)\<close>
     using tree2 by auto
-  hence \<open>interp_op (Move t1 p1 m1 c1) (interp_op (Move t2 p2 m2 c2) ([], tree)) =
+  hence \<open>apply_op (Move t1 p1 m1 c1) (apply_op (Move t2 p2 m2 c2) ([], tree)) =
          redo_op (LogMove t2 (get_parent tree c2) p2 m2 c2) ([LogMove t1 (get_parent tree c1) p1 m1 c1], tree1)\<close>
     using tree1 undo2 assms(1) by auto
   ultimately show ?thesis
     using tree12 by auto
 qed
 
-lemma interp_op_log_cons:
-  assumes \<open>interp_op (Move t1 p1 m1 c1) (log, tree) = (log2, tree2)\<close>
+lemma apply_op_log_cons:
+  assumes \<open>apply_op (Move t1 p1 m1 c1) (log, tree) = (log2, tree2)\<close>
   shows \<open>\<exists>logop rest. log2 = logop # rest \<and> t1 \<le> log_time logop\<close>
 proof(cases log)
   case Nil
@@ -815,11 +816,11 @@ next
   then show ?thesis
   proof(cases \<open>t1 < t2\<close>)
     case True
-    obtain tree1 log1 where tree1: \<open>interp_op (Move t1 p1 m1 c1) (rest, undo_op (logop, tree)) = (log1, tree1)\<close>
+    obtain tree1 log1 where tree1: \<open>apply_op (Move t1 p1 m1 c1) (rest, undo_op (logop, tree)) = (log1, tree1)\<close>
       by fastforce
     obtain tree12 where \<open>do_op (Move t2 p2 m2 c2, tree1) = (LogMove t2 (get_parent tree1 c2) p2 m2 c2, tree12)\<close>
       by simp
-    hence \<open>interp_op (Move t1 p1 m1 c1) (log, tree) = (LogMove t2 (get_parent tree1 c2) p2 m2 c2 # log1, tree12)\<close>
+    hence \<open>apply_op (Move t1 p1 m1 c1) (log, tree) = (LogMove t2 (get_parent tree1 c2) p2 m2 c2 # log1, tree12)\<close>
       using True local.Cons tree1 logop by auto
     then show ?thesis
       using True assms by auto
@@ -827,7 +828,7 @@ next
     case False
     obtain tree1 where tree1: \<open>do_op (Move t1 p1 m1 c1, tree) = (LogMove t1 (get_parent tree c1) p1 m1 c1, tree1)\<close>
       by simp
-    hence \<open>interp_op (Move t1 p1 m1 c1) (log, tree) =
+    hence \<open>apply_op (Move t1 p1 m1 c1) (log, tree) =
            (LogMove t1 (get_parent tree c1) p1 m1 c1 # log, tree1)\<close>
       using False local.Cons logop by auto
     then show ?thesis
@@ -835,15 +836,15 @@ next
   qed
 qed
 
-lemma interp_op_commute2:
+lemma apply_op_commute2:
   assumes \<open>t1 < t2\<close>
     and \<open>unique_parent tree\<close>
     and \<open>distinct ((map log_time log) @ [t1, t2])\<close>
-  shows \<open>interp_op (Move t2 p2 m2 c2) (interp_op (Move t1 p1 m1 c1) (log, tree)) =
-         interp_op (Move t1 p1 m1 c1) (interp_op (Move t2 p2 m2 c2) (log, tree))\<close>
+  shows \<open>apply_op (Move t2 p2 m2 c2) (apply_op (Move t1 p1 m1 c1) (log, tree)) =
+         apply_op (Move t1 p1 m1 c1) (apply_op (Move t2 p2 m2 c2) (log, tree))\<close>
 using assms proof(induction log arbitrary: tree)
   case Nil
-  then show ?case using interp_op_commute_base by metis
+  then show ?case using apply_op_commute_base by metis
 next
   case (Cons logop log)
   have parent0: \<open>unique_parent (undo_op (logop, tree))\<close>
@@ -865,21 +866,21 @@ next
       using Cons.prems(2) do_undo_op_inv by metis
     have \<open>\<not> t2 < t1\<close>
       using not_less_iff_gr_or_eq Cons.prems(1) by blast
-    hence \<open>interp_op (Move t2 p2 m2 c2) (interp_op (Move t1 p1 m1 c1) (logop # log, tree)) =
+    hence \<open>apply_op (Move t2 p2 m2 c2) (apply_op (Move t1 p1 m1 c1) (logop # log, tree)) =
            ([LogMove t2 (get_parent tree1 c2) p2 m2 c2, LogMove t1 (get_parent tree c1) p1 m1 c1, logop] @ log, tree12)\<close>
       using tree1 tree12 logop c1 by auto
     moreover have \<open>t3 < t2\<close>
       using c1 Cons.prems(1) by auto
-    hence \<open>interp_op (Move t2 p2 m2 c2) (logop # log, tree) = (LogMove t2 (get_parent tree c2) p2 m2 c2 # logop # log, tree2)\<close>
+    hence \<open>apply_op (Move t2 p2 m2 c2) (logop # log, tree) = (LogMove t2 (get_parent tree c2) p2 m2 c2 # logop # log, tree2)\<close>
       using tree2 logop by auto
-    hence \<open>interp_op (Move t1 p1 m1 c1) (interp_op (Move t2 p2 m2 c2) (logop # log, tree)) =
+    hence \<open>apply_op (Move t1 p1 m1 c1) (apply_op (Move t2 p2 m2 c2) (logop # log, tree)) =
            redo_op (LogMove t2 (get_parent tree c2) p2 m2 c2) (LogMove t1 (get_parent tree c1) p1 m1 c1 # logop # log, tree1)\<close>
       using Cons.prems(1) c1 logop tree1 undo2 by auto
     ultimately show ?thesis
       using tree12 by auto
   next
     case c2 (* t1 < t3 < t2 *)
-    obtain tree1 log1 where tree1: \<open>interp_op (Move t1 p1 m1 c1) (log, undo_op (logop, tree)) = (log1, tree1)\<close>
+    obtain tree1 log1 where tree1: \<open>apply_op (Move t1 p1 m1 c1) (log, undo_op (logop, tree)) = (log1, tree1)\<close>
       by fastforce
     obtain tree13 where tree13: \<open>do_op (Move t3 p3 m3 c3, tree1) = (LogMove t3 (get_parent tree1 c3) p3 m3 c3, tree13)\<close>
       by simp
@@ -889,36 +890,36 @@ next
       by simp
     hence undo2: \<open>undo_op (LogMove t2 (get_parent tree c2) p2 m2 c2, tree2) = tree\<close>
       by (metis Cons.prems(2) do_undo_op_inv)
-    have \<open>interp_op (Move t2 p2 m2 c2) (interp_op (Move t1 p1 m1 c1) (logop # log, tree)) =
+    have \<open>apply_op (Move t2 p2 m2 c2) (apply_op (Move t1 p1 m1 c1) (logop # log, tree)) =
            (LogMove t2 (get_parent tree13 c2) p2 m2 c2 # LogMove t3 (get_parent tree1 c3) p3 m3 c3 # log1, tree132)\<close>
       using c2 logop tree1 tree13 tree132 by auto
-    moreover have \<open>interp_op (Move t2 p2 m2 c2) (logop # log, tree) =
+    moreover have \<open>apply_op (Move t2 p2 m2 c2) (logop # log, tree) =
                    (LogMove t2 (get_parent tree c2) p2 m2 c2 # logop # log, tree2)\<close>
       using c2 logop tree2 by auto
-    hence \<open>interp_op (Move t1 p1 m1 c1) (interp_op (Move t2 p2 m2 c2) (logop # log, tree)) =
+    hence \<open>apply_op (Move t1 p1 m1 c1) (apply_op (Move t2 p2 m2 c2) (logop # log, tree)) =
            (LogMove t2 (get_parent tree13 c2) p2 m2 c2 # LogMove t3 (get_parent tree1 c3) p3 m3 c3 # log1, tree132)\<close>
       using assms(1) undo2 c2 logop tree1 tree13 tree132 by auto
     ultimately show ?thesis by simp
   next
     case c3 (* t1 < t2 < t3 *)
-    obtain tree1 log1 where tree1: \<open>interp_op (Move t1 p1 m1 c1) (log, undo_op (logop, tree)) = (log1, tree1)\<close>
+    obtain tree1 log1 where tree1: \<open>apply_op (Move t1 p1 m1 c1) (log, undo_op (logop, tree)) = (log1, tree1)\<close>
       by fastforce
     obtain tree13 where tree13: \<open>do_op (Move t3 p3 m3 c3, tree1) = (LogMove t3 (get_parent tree1 c3) p3 m3 c3, tree13)\<close>
       by simp
     hence undo13: \<open>undo_op (LogMove t3 (get_parent tree1 c3) p3 m3 c3, tree13) = tree1\<close>
     proof -
       have \<open>unique_parent tree1\<close>
-        by (meson interp_op_unique_parent parent0 tree1)
+        by (meson apply_op_unique_parent parent0 tree1)
       thus ?thesis
         using do_undo_op_inv tree13 by metis
     qed
-    obtain tree12 log12 where tree12: \<open>interp_op (Move t2 p2 m2 c2) (log1, tree1) = (log12, tree12)\<close>
+    obtain tree12 log12 where tree12: \<open>apply_op (Move t2 p2 m2 c2) (log1, tree1) = (log12, tree12)\<close>
       by fastforce
     obtain tree123 where tree123: \<open>do_op (Move t3 p3 m3 c3, tree12) = (LogMove t3 (get_parent tree12 c3) p3 m3 c3, tree123)\<close>
       by simp
-    obtain tree2 log2 where tree2: \<open>interp_op (Move t2 p2 m2 c2) (log, undo_op (logop, tree)) = (log2, tree2)\<close>
+    obtain tree2 log2 where tree2: \<open>apply_op (Move t2 p2 m2 c2) (log, undo_op (logop, tree)) = (log2, tree2)\<close>
       by fastforce
-    obtain tree21 log21 where tree21: \<open>interp_op (Move t1 p1 m1 c1) (log2, tree2) = (log21, tree21)\<close>
+    obtain tree21 log21 where tree21: \<open>apply_op (Move t1 p1 m1 c1) (log2, tree2) = (log21, tree21)\<close>
       by fastforce
     obtain tree213 where tree213: \<open>do_op (Move t3 p3 m3 c3, tree21) = (LogMove t3 (get_parent tree21 c3) p3 m3 c3, tree213)\<close>
       by simp
@@ -927,56 +928,56 @@ next
     hence undo23: \<open>undo_op (LogMove t3 (get_parent tree2 c3) p3 m3 c3, tree23) = tree2\<close>
     proof -
       have \<open>unique_parent tree2\<close>
-        by (meson interp_op_unique_parent parent0 tree2)
+        by (meson apply_op_unique_parent parent0 tree2)
       thus ?thesis
         using do_undo_op_inv tree23 by metis
     qed
-    have \<open>interp_op (Move t1 p1 m1 c1) (logop # log, tree) =
+    have \<open>apply_op (Move t1 p1 m1 c1) (logop # log, tree) =
            (LogMove t3 (get_parent tree1 c3) p3 m3 c3 # log1, tree13)\<close>
       using assms(1) c3 logop tree1 tree13 by auto
-    hence \<open>interp_op (Move t2 p2 m2 c2) (interp_op (Move t1 p1 m1 c1) (logop # log, tree)) =
+    hence \<open>apply_op (Move t2 p2 m2 c2) (apply_op (Move t1 p1 m1 c1) (logop # log, tree)) =
            (LogMove t3 (get_parent tree12 c3) p3 m3 c3 # log12, tree123)\<close>
       using c3 tree12 tree123 undo13 by auto
-    moreover have \<open>interp_op (Move t2 p2 m2 c2) (logop # log, tree) =
+    moreover have \<open>apply_op (Move t2 p2 m2 c2) (logop # log, tree) =
           (LogMove t3 (get_parent tree2 c3) p3 m3 c3 # log2, tree23)\<close>
       using c3 logop tree2 tree23 by auto
-    hence \<open>interp_op (Move t1 p1 m1 c1) (interp_op (Move t2 p2 m2 c2) (logop # log, tree)) =
+    hence \<open>apply_op (Move t1 p1 m1 c1) (apply_op (Move t2 p2 m2 c2) (logop # log, tree)) =
            (LogMove t3 (get_parent tree21 c3) p3 m3 c3 # log21, tree213)\<close>
       using assms(1) c3 undo23 tree21 tree213 by auto
-    moreover have \<open>interp_op (Move t2 p2 m2 c2) (interp_op (Move t1 p1 m1 c1) (log, undo_op (logop, tree))) =
-                   interp_op (Move t1 p1 m1 c1) (interp_op (Move t2 p2 m2 c2) (log, undo_op (logop, tree)))\<close>
+    moreover have \<open>apply_op (Move t2 p2 m2 c2) (apply_op (Move t1 p1 m1 c1) (log, undo_op (logop, tree))) =
+                   apply_op (Move t1 p1 m1 c1) (apply_op (Move t2 p2 m2 c2) (log, undo_op (logop, tree)))\<close>
       using Cons.IH Cons.prems(3) assms(1) parent0 by auto
     ultimately show ?thesis
       using tree1 tree12 tree123 tree2 tree21 tree213 by auto
   qed
 qed
 
-corollary interp_op_commute2I:
+corollary apply_op_commute2I:
   assumes \<open>unique_parent tree\<close>
     and \<open>distinct ((map log_time log) @ [t1, t2])\<close>
-    and \<open>interp_op (Move t1 p1 m1 c1) (log, tree) = (log1, tree1)\<close>
-    and \<open>interp_op (Move t2 p2 m2 c2) (log, tree) = (log2, tree2)\<close>
-  shows \<open>interp_op (Move t2 p2 m2 c2) (log1, tree1) = interp_op (Move t1 p1 m1 c1) (log2, tree2)\<close>
-proof (case_tac \<open>t1 < t2\<close>, metis assms interp_op_commute2)
+    and \<open>apply_op (Move t1 p1 m1 c1) (log, tree) = (log1, tree1)\<close>
+    and \<open>apply_op (Move t2 p2 m2 c2) (log, tree) = (log2, tree2)\<close>
+  shows \<open>apply_op (Move t2 p2 m2 c2) (log1, tree1) = apply_op (Move t1 p1 m1 c1) (log2, tree2)\<close>
+proof (case_tac \<open>t1 < t2\<close>, metis assms apply_op_commute2)
   assume \<open>\<not> t1 < t2\<close>
   hence \<open>t2 < t1\<close>
     using assms by force
   moreover have \<open>distinct ((map log_time log) @ [t2, t1])\<close>
     using assms by force
   ultimately show ?thesis
-    using assms interp_op_commute2 by metis
+    using assms apply_op_commute2 by metis
 qed
 
-lemma interp_op_timestamp:
+lemma apply_op_timestamp:
   assumes \<open>distinct ((map log_time log1) @ [t])\<close>
-    and \<open>interp_op (Move t p m c) (log1, tree1) = (log2, tree2)\<close>
+    and \<open>apply_op (Move t p m c) (log1, tree1) = (log2, tree2)\<close>
   shows \<open>distinct (map log_time log2) \<and> set (map log_time log2) = {t} \<union> set (map log_time log1)\<close>
 using assms proof(induction log1 arbitrary: tree1 log2 tree2)
   case Nil
   then show ?case by auto
 next
   case (Cons logop log)
-  obtain log3 tree3 where log3: \<open>interp_op (Move t p m c) (log, undo_op (logop, tree1)) = (log3, tree3)\<close>
+  obtain log3 tree3 where log3: \<open>apply_op (Move t p m c) (log, undo_op (logop, tree1)) = (log3, tree3)\<close>
     using prod.exhaust_sel by blast
   have \<open>distinct ((map log_time log) @ [t])\<close>
     using Cons.prems(1) by auto
@@ -989,7 +990,7 @@ next
       using log_op.exhaust by blast
     obtain tree4 where \<open>do_op (Move t2 p2 m2 c2, tree3) = (LogMove t2 (get_parent tree3 c2) p2 m2 c2, tree4)\<close>
       by simp
-    hence \<open>interp_op (Move t p m c) (logop # log, tree1) =
+    hence \<open>apply_op (Move t p m c) (logop # log, tree1) =
            (LogMove t2 (get_parent tree3 c2) p2 m2 c2 # log3, tree4)\<close>
       using logop log3 recursive_case by auto
     moreover from this have \<open>set (map log_time log2) = {t} \<union> set (map log_time (logop # log))\<close>
@@ -1002,7 +1003,7 @@ next
     case cons_case: False
     obtain tree4 where \<open>do_op (Move t p m c, tree1) = (LogMove t (get_parent tree1 c) p m c, tree4)\<close>
       by simp
-    hence \<open>interp_op (Move t p m c) (logop # log, tree1) =
+    hence \<open>apply_op (Move t p m c) (logop # log, tree1) =
            (LogMove t (get_parent tree1 c) p m c # logop # log, tree4)\<close>
       by (simp add: cons_case)
     moreover from this have \<open>set (map log_time log2) = {t} \<union> set (map log_time (logop # log))\<close>
@@ -1014,23 +1015,23 @@ next
   qed
 qed
 
-corollary interp_op_timestampI1:
-  assumes \<open>interp_op (Move t p m c) (log1, tree1) = (log2, tree2)\<close> \<open>distinct ((map log_time log1) @ [t])\<close>
+corollary apply_op_timestampI1:
+  assumes \<open>apply_op (Move t p m c) (log1, tree1) = (log2, tree2)\<close> \<open>distinct ((map log_time log1) @ [t])\<close>
   shows \<open>distinct (map log_time log2)\<close>
-  using assms interp_op_timestamp by metis
+  using assms apply_op_timestamp by metis
 
-corollary interp_op_timestampI2:
-  assumes \<open>interp_op (Move t p m c) (log1, tree1) = (log2, tree2)\<close> \<open>distinct ((map log_time log1) @ [t])\<close>
+corollary apply_op_timestampI2:
+  assumes \<open>apply_op (Move t p m c) (log1, tree1) = (log2, tree2)\<close> \<open>distinct ((map log_time log1) @ [t])\<close>
   shows \<open>set (map log_time log2) = {t} \<union> set (map log_time log1)\<close>
-  using assms interp_op_timestamp by metis
+  using assms apply_op_timestamp by metis
 
-lemma interp_ops_timestamps:
+lemma apply_ops_timestamps:
   assumes \<open>distinct (map move_time ops)\<close>
-    and \<open>interp_ops ops = (log, tree)\<close>
+    and \<open>apply_ops ops = (log, tree)\<close>
   shows \<open>distinct (map log_time log) \<and> set (map move_time ops) = set (map log_time log)\<close>
 using assms proof(induction ops arbitrary: log tree rule: List.rev_induct, simp)
   case (snoc oper ops)
-  obtain log1 tree1 where log1: \<open>interp_ops ops = (log1, tree1)\<close>
+  obtain log1 tree1 where log1: \<open>apply_ops ops = (log1, tree1)\<close>
     by fastforce
   hence IH: \<open>distinct (map log_time log1) \<and> set (map move_time ops) = set (map log_time log1)\<close>
     using snoc by auto
@@ -1039,28 +1040,28 @@ using assms proof(induction ops arbitrary: log tree rule: List.rev_induct, simp)
   moreover have \<open>distinct (map log_time log1 @ [move_time oper])\<close>
     using log1 snoc(1) snoc.prems(1) by force
   ultimately show ?case
-    by (metis (no_types) interp_op_timestamp interp_ops_step log1 operation.exhaust_sel snoc.prems(2))
+    by (metis (no_types) apply_op_timestamp apply_ops_step log1 operation.exhaust_sel snoc.prems(2))
 qed
 
-lemma interp_op_commute_last:
+lemma apply_op_commute_last:
   assumes \<open>distinct ((map move_time ops) @ [t1, t2])\<close>
-  shows \<open>interp_ops (ops @ [Move t1 p1 m1 c1, Move t2 p2 m2 c2]) =
-         interp_ops (ops @ [Move t2 p2 m2 c2, Move t1 p1 m1 c1])\<close>
+  shows \<open>apply_ops (ops @ [Move t1 p1 m1 c1, Move t2 p2 m2 c2]) =
+         apply_ops (ops @ [Move t2 p2 m2 c2, Move t1 p1 m1 c1])\<close>
 proof -
-  obtain log tree where interp_ops: \<open>interp_ops ops = (log, tree)\<close>
+  obtain log tree where apply_ops: \<open>apply_ops ops = (log, tree)\<close>
     by fastforce
   hence unique_parent: \<open>unique_parent tree\<close>
-    by (meson interp_ops_unique_parent)
+    by (meson apply_ops_unique_parent)
   have distinct_times: \<open>distinct ((map log_time log) @ [t1, t2])\<close>
-    using assms interp_ops interp_ops_timestamps by auto
-  have \<open>interp_ops (ops @ [Move t1 p1 m1 c1, Move t2 p2 m2 c2]) =
-        interp_op (Move t2 p2 m2 c2) (interp_op (Move t1 p1 m1 c1) (log, tree))\<close>
-    using interp_ops by (simp add: interp_ops_def)
-  also have \<open>... = interp_op (Move t1 p1 m1 c1) (interp_op (Move t2 p2 m2 c2) (log, tree))\<close>
+    using assms apply_ops apply_ops_timestamps by auto
+  have \<open>apply_ops (ops @ [Move t1 p1 m1 c1, Move t2 p2 m2 c2]) =
+        apply_op (Move t2 p2 m2 c2) (apply_op (Move t1 p1 m1 c1) (log, tree))\<close>
+    using apply_ops by (simp add: apply_ops_def)
+  also have \<open>... = apply_op (Move t1 p1 m1 c1) (apply_op (Move t2 p2 m2 c2) (log, tree))\<close>
   proof(cases \<open>t1 < t2\<close>)
     case True
     then show ?thesis
-      by (metis unique_parent distinct_times interp_op_commute2)
+      by (metis unique_parent distinct_times apply_op_commute2)
   next
     case False
     hence \<open>t2 < t1\<close>
@@ -1068,60 +1069,60 @@ proof -
     moreover have \<open>distinct ((map log_time log) @ [t2, t1])\<close>
       using distinct_times by auto
     ultimately show ?thesis
-      by (metis unique_parent interp_op_commute2)
+      by (metis unique_parent apply_op_commute2)
   qed
-  also have \<open>... = interp_ops (ops @ [Move t2 p2 m2 c2, Move t1 p1 m1 c1])\<close>
-    using interp_ops by (simp add: interp_ops_def)
+  also have \<open>... = apply_ops (ops @ [Move t2 p2 m2 c2, Move t1 p1 m1 c1])\<close>
+    using apply_ops by (simp add: apply_ops_def)
   ultimately show ?thesis
     by presburger
 qed
 
-lemma interp_op_commute_middle:
+lemma apply_op_commute_middle:
   assumes \<open>distinct (map move_time (xs @ ys @ [oper]))\<close>
-  shows \<open>interp_ops (xs @ ys @ [oper]) = interp_ops (xs @ [oper] @ ys)\<close>
+  shows \<open>apply_ops (xs @ ys @ [oper]) = apply_ops (xs @ [oper] @ ys)\<close>
 using assms proof(induction ys rule: List.rev_induct, simp)
   case (snoc y ys)
-  have \<open>interp_ops (xs @ [oper] @ ys @ [y]) = interp_op y (interp_ops (xs @ [oper] @ ys))\<close>
-    by (metis append.assoc interp_ops_step)
-  also have \<open>... = interp_op y (interp_ops (xs @ ys @ [oper]))\<close>
+  have \<open>apply_ops (xs @ [oper] @ ys @ [y]) = apply_op y (apply_ops (xs @ [oper] @ ys))\<close>
+    by (metis append.assoc apply_ops_step)
+  also have \<open>... = apply_op y (apply_ops (xs @ ys @ [oper]))\<close>
   proof -
     have \<open>distinct (map move_time (xs @ ys @ [oper]))\<close>
       using snoc.prems by auto
     then show ?thesis
       using snoc.IH by auto
   qed
-  also have \<open>... = interp_ops ((xs @ ys) @ [oper, y])\<close>
-    by (metis append.assoc append_Cons append_Nil interp_ops_step)
-  also have \<open>... = interp_ops ((xs @ ys) @ [y, oper])\<close>
+  also have \<open>... = apply_ops ((xs @ ys) @ [oper, y])\<close>
+    by (metis append.assoc append_Cons append_Nil apply_ops_step)
+  also have \<open>... = apply_ops ((xs @ ys) @ [y, oper])\<close>
   proof -
     have \<open>distinct ((map move_time (xs @ ys)) @ [move_time y, move_time oper])\<close>
       using snoc.prems by auto
     thus ?thesis
-      using interp_op_commute_last by (metis operation.exhaust_sel)
+      using apply_op_commute_last by (metis operation.exhaust_sel)
   qed
   ultimately show ?case
     by simp
 qed
 
-theorem interp_ops_commutes:
+theorem apply_ops_commutes:
   assumes \<open>set ops1 = set ops2\<close>
     and \<open>distinct (map move_time ops1)\<close>
     and \<open>distinct (map move_time ops2)\<close>
-  shows \<open>interp_ops ops1 = interp_ops ops2\<close>
+  shows \<open>apply_ops ops1 = apply_ops ops2\<close>
 using assms proof(induction ops1 arbitrary: ops2 rule: List.rev_induct, simp)
   case (snoc oper ops)
   then obtain pre suf where pre_suf: \<open>ops2 = pre @ [oper] @ suf\<close>
     by (metis append_Cons append_Nil in_set_conv_decomp)
   hence \<open>set ops = set (pre @ suf)\<close>
     using snoc.prems distinct_map distinct_list_pick1 by metis
-  hence IH: \<open>interp_ops ops = interp_ops (pre @ suf)\<close>
+  hence IH: \<open>apply_ops ops = apply_ops (pre @ suf)\<close>
     using pre_suf snoc.IH snoc.prems by auto
   moreover have \<open>distinct (map move_time (pre @ suf @ [oper]))\<close>
     using pre_suf snoc.prems(3) by auto
-  moreover from this have \<open>interp_ops (pre @ suf @ [oper]) = interp_ops (pre @ [oper] @ suf)\<close>
-    using interp_op_commute_middle by blast
-  ultimately show \<open>interp_ops (ops @ [oper]) = interp_ops ops2\<close>
-    by (metis append_assoc interp_ops_step pre_suf)
+  moreover from this have \<open>apply_ops (pre @ suf @ [oper]) = apply_ops (pre @ [oper] @ suf)\<close>
+    using apply_op_commute_middle by blast
+  ultimately show \<open>apply_ops (ops @ [oper]) = apply_ops ops2\<close>
+    by (metis append_assoc apply_ops_step pre_suf)
 qed
 
 section\<open>Code generation: an efficient implementation\<close>
@@ -1437,21 +1438,21 @@ fun efficient_redo_op :: \<open>('t, 'n, 'm) log_op \<Rightarrow>
           (let (op2, tree2) = efficient_do_op (Move t p m c, tree) in
              (op2#ops, tree2))\<close>
 
-fun efficient_interp_op :: \<open>('t::{linorder}, 'n, 'm) operation \<Rightarrow>
+fun efficient_apply_op :: \<open>('t::{linorder}, 'n, 'm) operation \<Rightarrow>
               ('t, 'n, 'm) log_op list \<times> ('n::{hashable}, 'm \<times> 'n) hm \<Rightarrow>
             ('t, 'n, 'm) log_op list \<times> ('n, 'm \<times> 'n) hm\<close>
-  where \<open>efficient_interp_op op1 ([], tree1) =
+  where \<open>efficient_apply_op op1 ([], tree1) =
           (let (op2, tree2) = efficient_do_op (op1, tree1)
             in ([op2], tree2))\<close>
-      | \<open>efficient_interp_op op1 (logop#ops, tree1) =
+      | \<open>efficient_apply_op op1 (logop#ops, tree1) =
           (if move_time op1 < log_time logop
-            then efficient_redo_op logop (efficient_interp_op op1 (ops, efficient_undo_op (logop, tree1)))
+            then efficient_redo_op logop (efficient_apply_op op1 (ops, efficient_undo_op (logop, tree1)))
               else let (op2, tree2) = efficient_do_op (op1, tree1) in (op2 # logop # ops, tree2))\<close>
 
-definition efficient_interp_ops :: \<open>('t::{linorder}, 'n::{hashable}, 'm) operation list \<Rightarrow>
+definition efficient_apply_ops :: \<open>('t::{linorder}, 'n::{hashable}, 'm) operation list \<Rightarrow>
         ('t, 'n, 'm) log_op list \<times> ('n::{hashable}, 'm \<times> 'n) hm\<close>
-  where \<open>efficient_interp_ops ops \<equiv>
-      foldl (\<lambda>state oper. efficient_interp_op oper state) ([], (hm.empty ())) ops\<close>
+  where \<open>efficient_apply_ops ops \<equiv>
+      foldl (\<lambda>state oper. efficient_apply_op oper state) ([], (hm.empty ())) ops\<close>
 
 text\<open>Any abstract set that is simulated by a hash-map must necessarily have the
      @{term unique_parent} property:\<close>
@@ -1693,17 +1694,17 @@ using assms proof(cases \<open>oper\<close>)
 qed
 
 (* this proof, lol *)
-lemma efficient_interp_op_refines:
+lemma efficient_apply_op_refines:
   assumes \<open>t \<preceq> T\<close>
-    and \<open>efficient_interp_op oper (log, t) = (log1, u)\<close>
-    and \<open>interp_op oper (log, T) = (log2, U)\<close>
+    and \<open>efficient_apply_op oper (log, t) = (log1, u)\<close>
+    and \<open>apply_op oper (log, T) = (log2, U)\<close>
   shows \<open>log1 = log2 \<and> u \<preceq> U\<close>
 using assms
   apply(subgoal_tac \<open>unique_parent T\<close>)
 prefer 2
   apply(force intro: refines_unique_parent)
   apply(induction log arbitrary: T t log1 log2 u U)
-  apply(simp only: efficient_interp_op.simps interp_op.simps)
+  apply(simp only: efficient_apply_op.simps apply_op.simps)
   apply(intro conjI)
   apply(clarsimp simp add: Let_def split!: prod.split_asm)
   apply(erule conjE[OF efficient_do_op_refines], force, force, force)
@@ -1711,8 +1712,8 @@ prefer 2
   apply(erule conjE[OF efficient_do_op_refines], force, force, force)
   apply clarsimp
   apply(case_tac \<open>move_time oper < log_time a\<close>; clarsimp)
-  apply(case_tac \<open>efficient_interp_op oper (log, efficient_undo_op (a, t))\<close>)
-  apply(case_tac \<open>interp_op oper (log, undo_op (a, T))\<close>)
+  apply(case_tac \<open>efficient_apply_op oper (log, efficient_undo_op (a, t))\<close>)
+  apply(case_tac \<open>apply_op oper (log, undo_op (a, T))\<close>)
   apply(subgoal_tac \<open>ab = aa \<and> b \<preceq> ba\<close>)
   apply(erule_tac x=\<open>undo_op (a, T)\<close> in meta_allE)
   apply(erule_tac x=\<open>efficient_undo_op (a, t)\<close> in meta_allE)
@@ -1752,26 +1753,26 @@ defer
   apply(rule undo_op_unique_parent_variant, assumption, force)
   done
 
-text\<open>The internal workings of abstract and concrete implementations of the @{term interp_ops}
+text\<open>The internal workings of abstract and concrete implementations of the @{term apply_ops}
      function map related states to related states, and produce identical logs, when passed
      identical lists of actions to perform.
 
-     Note this lemma is necessary as the @{term interp_ops} function specifies a particular starting
-     state (the empty state) to start the iterated application of the @{term interp_op} function
+     Note this lemma is necessary as the @{term apply_ops} function specifies a particular starting
+     state (the empty state) to start the iterated application of the @{term apply_op} function
      from, meaning that an inductive proof using this definition directly becomes impossible, as the
      inductive hypothesis will be over constrained in the step case.  By introducing this lemma, we
      show that the required property holds for any starting states (as long as they are related by
      the simulation relation) and then specialise to the empty starting state in the next lemma,
      below.\<close>
-lemma efficient_interp_ops_refines_internal:
-  assumes \<open>foldl (\<lambda>state oper. efficient_interp_op oper state) (log, t) xs = (log1, u)\<close>
-    and \<open>foldl (\<lambda>state oper. interp_op oper state) (log, T) xs = (log2, U)\<close>
+lemma efficient_apply_ops_refines_internal:
+  assumes \<open>foldl (\<lambda>state oper. efficient_apply_op oper state) (log, t) xs = (log1, u)\<close>
+    and \<open>foldl (\<lambda>state oper. apply_op oper state) (log, T) xs = (log2, U)\<close>
     and \<open>t \<preceq> T\<close>
   shows \<open>log1 = log2 \<and> u \<preceq> U\<close>
 using assms proof(induction xs arbitrary: log log1 log2 t T u U)
   case Nil
-  assume \<open>foldl (\<lambda>state oper. efficient_interp_op oper state) (log, t) [] = (log1, u)\<close>
-    and \<open>interp_ops' [] (log, T) = (log2, U)\<close>
+  assume \<open>foldl (\<lambda>state oper. efficient_apply_op oper state) (log, t) [] = (log1, u)\<close>
+    and \<open>apply_ops' [] (log, T) = (log2, U)\<close>
     and *: \<open>t \<preceq> T\<close>
   from this have \<open>log = log2\<close> and \<open>T = U\<close> and \<open>log = log1\<close> and \<open>t = u\<close>
     by auto
@@ -1781,66 +1782,66 @@ next
   case (Cons x xs)
   fix xs :: \<open>('a, 'b, 'c) operation list\<close> and x log log1 log2 t T u U
   assume IH: \<open>\<And>log log1 log2 t T u U.
-           foldl (\<lambda>state oper. efficient_interp_op oper state) (log, t) xs = (log1, u) \<Longrightarrow>
-           interp_ops' xs (log, T) = (log2, U) \<Longrightarrow> t \<preceq> T \<Longrightarrow> log1 = log2 \<and> u \<preceq> U\<close>
-    and 1: \<open>foldl (\<lambda>state oper. efficient_interp_op oper state) (log, t) (x#xs) = (log1, u)\<close>
-    and 2: \<open>interp_ops' (x#xs) (log, T) = (log2, U)\<close>
+           foldl (\<lambda>state oper. efficient_apply_op oper state) (log, t) xs = (log1, u) \<Longrightarrow>
+           apply_ops' xs (log, T) = (log2, U) \<Longrightarrow> t \<preceq> T \<Longrightarrow> log1 = log2 \<and> u \<preceq> U\<close>
+    and 1: \<open>foldl (\<lambda>state oper. efficient_apply_op oper state) (log, t) (x#xs) = (log1, u)\<close>
+    and 2: \<open>apply_ops' (x#xs) (log, T) = (log2, U)\<close>
     and 3: \<open>t \<preceq> T\<close>
-  obtain log1' log2' U' u' where 4: \<open>efficient_interp_op x (log, t) = (log1', u')\<close>
-      and 5: \<open>interp_op x (log, T) = (log2', U')\<close>
+  obtain log1' log2' U' u' where 4: \<open>efficient_apply_op x (log, t) = (log1', u')\<close>
+      and 5: \<open>apply_op x (log, T) = (log2', U')\<close>
     by fastforce
   moreover from this have \<open>log1' = log2'\<close> and \<open>u' \<preceq> U'\<close>
-    using efficient_interp_op_refines[OF 3] by blast+
-  moreover have \<open>foldl (\<lambda>state oper. efficient_interp_op oper state) (log1', u') xs = (log1, u)\<close>
+    using efficient_apply_op_refines[OF 3] by blast+
+  moreover have \<open>foldl (\<lambda>state oper. efficient_apply_op oper state) (log1', u') xs = (log1, u)\<close>
     using 1 and 4 by simp
-  moreover have \<open>interp_ops' xs (log2', U') = (log2, U)\<close>
+  moreover have \<open>apply_ops' xs (log2', U') = (log2, U)\<close>
     using 2 and 5 by simp
   ultimately show \<open>log1 = log2 \<and> u \<preceq> U\<close>
     by(auto simp add: IH)
 qed
 
-text\<open>The efficient and abstract versions of @{term interp_ops} produce identical operation logs and
+text\<open>The efficient and abstract versions of @{term apply_ops} produce identical operation logs and
      produce related concrete and abstract states:\<close>
-lemma efficient_interp_ops_refines:
-  assumes 1: \<open>efficient_interp_ops opers = (log1, u)\<close>
-    and 2: \<open>interp_ops opers = (log2, U)\<close>
+lemma efficient_apply_ops_refines:
+  assumes 1: \<open>efficient_apply_ops opers = (log1, u)\<close>
+    and 2: \<open>apply_ops opers = (log2, U)\<close>
   shows \<open>log1 = log2 \<and> u \<preceq> U\<close>
 proof -
   have \<open>hm.empty () \<preceq> {}\<close>
     by auto
-  moreover have \<open>foldl (\<lambda>state oper. efficient_interp_op oper state) ([], hm.empty ()) opers = (log1, u)\<close>
-    using 1 by(auto simp add: efficient_interp_ops_def)
-  moreover have \<open>foldl (\<lambda>state oper. interp_op oper state) ([], {}) opers = (log2, U)\<close>
-    using 2 by(auto simp add: interp_ops_def)
+  moreover have \<open>foldl (\<lambda>state oper. efficient_apply_op oper state) ([], hm.empty ()) opers = (log1, u)\<close>
+    using 1 by(auto simp add: efficient_apply_ops_def)
+  moreover have \<open>foldl (\<lambda>state oper. apply_op oper state) ([], {}) opers = (log2, U)\<close>
+    using 2 by(auto simp add: apply_ops_def)
   moreover have \<open>log1 = log2\<close> and \<open>u \<preceq> U\<close>
-    using calculation efficient_interp_ops_refines_internal by blast+
+    using calculation efficient_apply_ops_refines_internal by blast+
   ultimately show \<open>?thesis\<close>
     by auto
 qed
 
 text\<open>The main correctness theorem for the efficient algorithms.  This follows the
-     @{thm interp_ops_commutes} theorem for the abstract algorithms with one significant difference:
-     the states obtained from interpreting the two lists of operations, @{term ops1} and
+     @{thm apply_ops_commutes} theorem for the abstract algorithms with one significant difference:
+     the states obtained from applyreting the two lists of operations, @{term ops1} and
      @{term ops2}, are no longer identical (the hash-maps may have a different representation in
      memory, for instance), but contain the same set of key-value bindings.  If we take equality of
      finite maps (hash-maps included) to be extensional---i.e. two finite maps are equal when they
      contain the same key-value bindings---then this theorem coincides exactly with the
-     @{thm interp_ops_commutes}:\<close>
-theorem efficient_interp_ops_commutes:
+     @{thm apply_ops_commutes}:\<close>
+theorem efficient_apply_ops_commutes:
   assumes 1: \<open>set ops1 = set ops2\<close>
     and 2: \<open>distinct (map move_time ops1)\<close>
     and 3: \<open>distinct (map move_time ops2)\<close>
-    and 4: \<open>efficient_interp_ops ops1 = (log1, t)\<close>
-    and 5: \<open>efficient_interp_ops ops2 = (log2, u)\<close>
+    and 4: \<open>efficient_apply_ops ops1 = (log1, t)\<close>
+    and 5: \<open>efficient_apply_ops ops2 = (log2, u)\<close>
   shows \<open>log1 = log2 \<and> hm.lookup c t = hm.lookup c u\<close>
 proof -
-  from 1 2 3 have \<open>interp_ops ops1 = interp_ops ops2\<close>
-    using interp_ops_commutes by auto
-  from this obtain log1' log2' T U where 6: \<open>interp_ops ops1 = (log1', T)\<close>
-      and 7: \<open>interp_ops ops2 = (log2', U)\<close> and 8: \<open>log1' = log2'\<close> and 9: \<open>T = U\<close>
+  from 1 2 3 have \<open>apply_ops ops1 = apply_ops ops2\<close>
+    using apply_ops_commutes by auto
+  from this obtain log1' log2' T U where 6: \<open>apply_ops ops1 = (log1', T)\<close>
+      and 7: \<open>apply_ops ops2 = (log2', U)\<close> and 8: \<open>log1' = log2'\<close> and 9: \<open>T = U\<close>
     by fastforce
   moreover from 4 5 6 7 have \<open>log1 = log1'\<close> and \<open>log2 = log2'\<close> and \<open>t \<preceq> T\<close> and \<open>u \<preceq> U\<close>
-    using efficient_interp_ops_refines by force+
+    using efficient_apply_ops_refines by force+
   moreover from 8 have \<open>log1 = log2\<close>
     by(simp add: calculation)
   moreover have \<open>hm.lookup c t = hm.lookup c u\<close>
@@ -1859,27 +1860,27 @@ text\<open>Check that all of the efficient algorithms produce executable code fo
      bottom.  (View it in the Output buffer of the Isabelle/JEdit IDE.)\<close>
 
 export_code efficient_ancestor efficient_do_op efficient_undo_op efficient_redo_op
-  efficient_interp_op efficient_interp_ops in SML
+  efficient_apply_op efficient_apply_ops in SML
 export_code efficient_ancestor efficient_do_op efficient_undo_op efficient_redo_op
-  efficient_interp_op efficient_interp_ops in Scala
+  efficient_apply_op efficient_apply_ops in Scala
 export_code efficient_ancestor efficient_do_op efficient_undo_op efficient_redo_op
-  efficient_interp_op efficient_interp_ops in OCaml
+  efficient_apply_op efficient_apply_ops in OCaml
 export_code efficient_ancestor efficient_do_op efficient_undo_op efficient_redo_op
-  efficient_interp_op efficient_interp_ops in Haskell
+  efficient_apply_op efficient_apply_ops in Haskell
 
 text\<open>Without resorting to saving the generated code above to a separate file and feeding them into
      an SML/Scala/OCaml/Haskell compiler, as appropriate, we can show that this code compiles and
      executes relatively quickly from within Isabelle itself, by making use of Isabelle's
      quotations/anti-quotations, and its tight coupling with the underlying PolyML process.
 
-     First define a @{term unit_test} definition that makes use of our @{term efficient_interp_ops}
+     First define a @{term unit_test} definition that makes use of our @{term efficient_apply_ops}
      function on a variety of inputs:\<close>
 
 definition unit_test :: \<open>((nat, nat, nat) log_op list \<times> (nat, nat \<times> nat) HashMap.hashmap) list\<close>
   where \<open>unit_test \<equiv>
-          [ efficient_interp_ops []
-          , efficient_interp_ops [Move 1 0 0 0]
-          , efficient_interp_ops [Move 1 0 0 0, Move 3 2 2 2, Move 2 1 1 1]
+          [ efficient_apply_ops []
+          , efficient_apply_ops [Move 1 0 0 0]
+          , efficient_apply_ops [Move 1 0 0 0, Move 3 2 2 2, Move 2 1 1 1]
           ]\<close>
 
 text\<open>Then, we can use @{command ML_val} to ask Isabelle to:
